barrier/parameter.v
@@ -1,4 +1,0 @@
-Require Export barrier.heap_lang.
-Require Import iris.parameter.
-
-Canonical Structure Σ := iParam_const heap_lang unitRA.
